* Revision of the Ravenscar MoC

src/MoC/ravenscar.v
@@ -29,49 +29,173 @@
  *
  * DM21-0762
 ***)
-(**
+
+(*|
+******************************
+Ravenscar Model of Computation
+******************************
+
 In this module, we provide a formalization of the Ravenscar Ada profile.
-It follows the formalization proposed in
 
-Irfan Hamid, Elie Najm:
-Operational Semantics of Ada Ravenscar. Ada-Europe 2008: 44-58
-https://doi.org/10.1007/978-3-540-68624-8_4
+|*)
 
-Nice readings
-
-Yves Bertot. Theorem proving support in programming language semantics.
-[Research Report] RR- 6242, INRIA. 2007, pp.23. inria-00160309v2
-
-Yves Bertot. Semantics for programming languages with Coq encodings:
-First part: natural semantics. Master. France. 2015. cel-01130272
-
-*)
-
-Set Implicit Arguments.
-Require Import Coq.Init.Datatypes.
-Require Import Oqarina.core.identifiers.
+(*| .. coq:: none |*)
+Require Import Coq.Bool.Bool.
+Require Import Coq.Program.Equality.
+Require Import Coq.Relations.Relation_Definitions.
+Require Import Coq.Relations.Relation_Operators.
+Require Import Coq.Sorting.Permutation.
+Require Import Lia.
 Require Import List.
 Import ListNotations. (* from List *)
 
-(** A %\coqdocvar{seq_program}% denotes a sequence of code
-statements. By definition, it should not hold any calls to concurrent
-API. *)
+Require Import Oqarina.CoqExt.all.
 
-Definition seq_program := Set.
+Require Import Oqarina.core.all.
+Require Import Oqarina.coq_utils.all.
+Require Import Oqarina.formalisms.Expressions.all.
+Import NaturalTime.
 
-Definition Simple_Program : seq_program := Empty_set.
+Set Implicit Arguments.
+(*| .. coq:: |*)
+
+(*|
+Definitions
+===========
+
+|*)
 
 (** priority concept. *)
 
 Definition priority := nat.
 
-(** time concept. *)
+(*|
 
-Definition time := nat.
+Sequential programs
+-------------------
 
-(**
+A Ravenscar sequential program is reduced to a set of basic statements mimicking the imperative nature of an Ada program: XXX
 
-An Ada protected object is similar to a Hoard monitor or a Java Synchronized inteface:
+|*)
+
+Inductive statements : Type :=
+  (* A sequential execution step *)
+  | COMP  (WCET : Time)
+
+  (* Operations on protected objects *)
+  | PO_FUNCTION (po : identifier) (op : identifier)
+  | PO_ENTRY (po : identifier) (op : identifier)
+
+  (* Delay until some time *)
+  | DELAY_UNTIL_NEXT_PERIOD
+
+  (* Sequence of statements *)
+  | SEQ (s1: statements) (s2: statements)
+
+  (* While b is true, execute s1 *)
+  | WHILE (b: bexp) (s: statements)
+
+  | SKIP.
+
+Infix ";;" := SEQ (at level 80, right associativity).
+
+(*| * Example of Ravenscar programs |*)
+
+Example A_Program := COMP 1 ;; SKIP.
+
+Example Ravenscar_Cyclic_Program := WHILE TRUE (COMP 2 ;;
+                                                DELAY_UNTIL_NEXT_PERIOD).
+
+(*|
+
+Ravenscar tasks
+---------------
+
+An Ada task under the Ravenscar profile is uniquely defined by the tuple
+%(priority, period, WCET)%
+
+|*)
+
+Inductive task_kind :=
+  | PERIODIC | SPORADIC | BACKGROUND.
+
+Inductive task_state :=
+  | READY | RUNNING | IDLE | BLOCKED.
+
+Scheme Equality for task_state.
+
+Inductive task :=
+  | Task : task_kind ->
+          identifier ->
+          priority ->
+          Time -> (* period / MIAT *)
+          statements -> task.
+
+Record thread_state := {
+  th_period : Time ;      (* period of the thread*)
+  th_state : task_state ; (* current state *)
+  th_cet : Time ;         (* compute execution time clock*)
+  th_next_dispatch : Time (* time of the next dispatch *)
+}.
+
+Definition Dummy_thread_state := {|
+  th_period := 0 ;
+  th_state := RUNNING;
+  th_cet := 0 ;
+  th_next_dispatch := 0;
+|}.
+
+Definition set_thread_state (ts : thread_state) (state : task_state) := {|
+  th_state := state ;
+  th_period := ts.(th_period) ;
+  th_cet := ts.(th_cet) ;
+  th_next_dispatch := ts.(th_next_dispatch) |}.
+
+Definition reset_thread_cet (ts : thread_state) := {|
+  th_state := ts.(th_state) ;
+  th_period := ts.(th_period) ;
+  th_cet := 0 ;
+  th_next_dispatch := ts.(th_next_dispatch) |}.
+
+Definition ICET (s: statements) : nat :=
+  match s with
+  | COMP t => t
+  | PO_FUNCTION _ _ | PO_ENTRY _ _ => 0
+  | DELAY_UNTIL_NEXT_PERIOD => 0
+  | SKIP => 0
+  | SEQ _ _ => 0
+  | WHILE _ _ => 0
+  end.
+
+Definition Update_CET (st: thread_state) (s : statements) :=
+  {|
+    th_state := th_state st ;
+    th_period := th_period st ;
+    th_cet := th_cet st + (ICET s) ;
+    th_next_dispatch := st.(th_next_dispatch)
+  |}.
+
+Definition Set_Next_Dispatch_Time (st : thread_state) :=
+  {|
+    th_state := IDLE ;
+    th_period := th_period st ;
+    th_cet := th_cet st ;
+    th_next_dispatch :=
+      (th_next_dispatch st) + (th_period st)
+  |}.
+
+(*| We define an idle task as a background task with the lowest priority. It does nothin but waste CPU. |*)
+
+Definition IDLE_TASK :=
+  Task BACKGROUND (Id "Idle") 0 0 SKIP.
+
+(** XXX trivial checks on well-formedness possible here also ..*)
+
+(*|
+Ravenscar Protected Object
+--------------------------
+
+An Ada protected object is similar to a Hoare monitor or a Java Synchronized inteface:
 it is a collection of protected operations. There are four categories:
 
 – PO_Set: sets a value to a protected object PO,
@@ -83,141 +207,188 @@ a procedure (write lock) or a function (read lock)
 
 *)
 
+Definition po_state : Type := identifier -> Time.
+
 Inductive protected_operation :=
-| PO_Get : identifier -> seq_program -> protected_operation
-| PO_Set : identifier -> seq_program -> protected_operation
-| PO_Send : identifier -> seq_program -> protected_operation
-| PO_Wait : identifier -> seq_program -> protected_operation.
+| PO_Function : identifier -> statements -> protected_operation
+| PO_Entry : identifier -> statements-> protected_operation.
 
 Inductive protected_object :=
-| Protected_Object : identifier -> priority -> list protected_operation -> protected_object.
+| Protected_Object : identifier ->
+                     priority ->
+                     list protected_operation -> protected_object.
 
 Definition A_PO :=
   Protected_Object (Id "A_PO") 42
-    [ (PO_Get (Id "get") Simple_Program ) ;
-      (PO_Set (Id "set") Simple_Program)].
+    [ (PO_Function (Id "set") A_Program ) ;
+      (PO_Entry (Id "get") A_Program)].
 
-(**
-    A Ravenscar profile is reduced to a set of basic statements: XXX
+(*|
+Legal Ravenscar programs
+------------------------
 
-    *)
+We distinguish three cases of legal Ravenacar programs:
 
-Inductive statements : Type :=
-| COMP                                        (* A sequential execution step *)
-| PO_GET (po : identifier) (op : identifier)  (* Operations on protected objects *)
-| PO_SET (po : identifier) (op : identifier)
-| PO_SEND (po : identifier) (op : identifier)
-| PO_WAIT (po : identifier) (op : identifier)
-| DELAY_UNTIL (t : nat)                       (* delay until some time *)
-| SEQ (s1: statements) (s2: statements)       (* Sequence of statements *)
-| RET.
+* periodic body
+* sporadic body
+* protected operation
 
-Infix ";;" := SEQ (at level 80, right associativity).
+For each situation, we define a correspoding legality rule and shows it is decidable.
+|*)
 
-Definition A_Program := COMP ;; RET.
-Definition Ravenscar_Cyclic_Program := COMP ;;
-                                       PO_GET (Id "A_PO") (Id "get") ;;
-                                       DELAY_UNTIL 10.
+(*|  A legal periodic body (PB) has the form
+    PB := comp; PB | Set( _ ); PB | Get( _ ); PB | Send Event( _ ); PB | delay until
+|*)
 
-(** A legal periodic body (PB) has the form
-    PB := comp; PB | Set( _ ); PB | Get( _ ); PB | Send Event( _ ); PB | delay until *)
-
-Fixpoint Legal_Periodic_Body (p : statements)  :=
+Fixpoint Legal_Periodic_Body (p : statements) :=
   match p with
-  (* DELAY_UNTIL is the last statement *)
-  | COMP => False | PO_GET _ _ => False | PO_SET _ _ => False
-  | PO_SEND _ _ => False | PO_WAIT _ _ => False | RET => False
-  | DELAY_UNTIL _ => True
+  (* Atomic statements are always valid *)
+  | COMP _ | PO_FUNCTION _ _  => True (* XXX *)
+  | SKIP | DELAY_UNTIL_NEXT_PERIOD | WHILE _ _ => True
 
-  (* COMP, PO_GET, PO_SET, and PO_SENT are accepted *)
-  | COMP ;; s2 => Legal_Periodic_Body s2
-  | PO_GET _ _ ;; s2 => Legal_Periodic_Body s2
-  | PO_SET _ _ ;; s2 => Legal_Periodic_Body s2
-  | PO_SEND _ _ ;; s2 => Legal_Periodic_Body s2
-  (* PO_WAIT and RET are rejected *)
-  | PO_WAIT _ _ ;; _ => False
-  | RET ;; _ => False
-  (* DELAY_UNTIL cannot be in a sequence *)
-  | DELAY_UNTIL  _ ;; _ => False
+  (* Sequences of statements:
+    - COMP, PO_GET, PO_SET, and PO_SENT are accepted *)
+
+  (* PO_ENTRY and RET are rejected *)
+  | PO_ENTRY _ _ => False
+
+  (* DELAY_UNTIL_NEXT_PERIOD cannot be in a sequence, it can only be the last element *)
+  | DELAY_UNTIL_NEXT_PERIOD  ;; _ => False
 
   (* Iteration *)
-  | (s1 ;; s2) ;; s3 => Legal_Periodic_Body s1 /\ Legal_Periodic_Body s2
-                        /\ Legal_Periodic_Body s3
-  end.
+  | SEQ s1 s2 =>  Legal_Periodic_Body s1 /\ Legal_Periodic_Body s2
+end.
 
-(**
+Lemma Legal_Periodic_Body_dec: forall p,
+  { Legal_Periodic_Body p } + { ~ Legal_Periodic_Body p }.
+Proof.
+  induction p ; simpl ; auto.
+  destruct p1 ; auto ;
+  apply dec_sumbool_and ; auto.
+Qed.
 
-A legal Sporadic Body has the form
-    SB := Get Event ; PB
+Ltac prove_Legal_body := compute ; trivial ; auto.
 
-*)
+Fact Legal_Periodic_Body_A_Program : Legal_Periodic_Body A_Program.
+Proof.
+  prove_Legal_body.
+Qed.
 
-Fixpoint Legal_Sporadic_Body (p : statements)  :=
+Fact Legal_Periodic_Body_Ravenscar_Cyclic_Program :
+  Legal_Periodic_Body Ravenscar_Cyclic_Program.
+Proof.
+  prove_Legal_body.
+Qed.
+
+(*| XXX |*)
+
+Definition Legal_Sporadic_Body (p : statements)  :=
   match p with
   (* PO_WAIT is the first statement *)
-  | PO_WAIT _ _ ;; s2 => Legal_Periodic_Body s2
+  | PO_ENTRY _ _ ;; s2 => Legal_Periodic_Body s2
 
-  (* because the precedent rule exits to execute Legal_Periodic_Bodym the other
+  (* because the precedent rule exits to execute Legal_Periodic_Body, the other
      combination should be false *)
-  | COMP ;; _ => False | PO_GET _ _ ;; _ => False | PO_SET _ _ ;; _ => False
-  | PO_SEND _ _ ;; _ => False | RET ;; _ => False
-  | DELAY_UNTIL _ ;; _ => False
+  | _ => False
+end.
 
-  | COMP => False | PO_GET _ _ => False | PO_SET _ _ => False
-  | PO_SEND _ _ => False | PO_WAIT _ _ => True | RET => False
-  | DELAY_UNTIL _ => False
+Lemma Legal_Sporadic_Body_dec: forall p,
+  { Legal_Sporadic_Body p } + { ~ Legal_Sporadic_Body p }.
+Proof.
+  induction p ; simpl ; auto.
+  destruct p1 ; auto.
+  apply Legal_Periodic_Body_dec.
+Qed.
+
+(*||*)
+Fixpoint Legal_PO_Body (p : statements) :=
+  match p with
+  (* Atomic statements are always valid *)
+  | COMP _  | SKIP   | WHILE _ _ => True
+
+  (* Sequences of statements:
+    - COMP, PO_GET, PO_SET, and PO_SENT are accepted *)
+
+  (* PO_ENTRY and RET are rejected *)
+  | PO_FUNCTION _ _  => False (* XXX *)
+  | PO_ENTRY _ _ => False
+
+  (* DELAY_UNTIL_NEXT_PERIOD cannot be in a sequence, it can only be the last element *)
+  | DELAY_UNTIL_NEXT_PERIOD  => False
 
   (* Iteration *)
-  | (s1 ;; s2) ;; s3 => Legal_Sporadic_Body s1 /\ Legal_Periodic_Body s2
-                        /\ Legal_Periodic_Body s3
+  | SEQ s1 s2 =>  Legal_PO_Body s1 /\ Legal_PO_Body s2
+end.
+
+Lemma Legal_PO_Body_dec: forall p,
+  { Legal_PO_Body p } + { ~ Legal_PO_Body p }.
+Proof.
+  induction p ; simpl ; auto.
+  apply dec_sumbool_and ; auto.
+Qed.
+
+Definition Legal_protected_operation (p : protected_operation) :=
+  match p with
+    | PO_Function _ s => Legal_PO_Body s
+    | PO_Entry _ s => Legal_PO_Body s
   end.
 
-(**
+  Lemma Legal_protected_operation_dec: forall p,
+  { Legal_protected_operation p } + { ~ Legal_protected_operation p }.
+Proof.
 
-An Ada task under the Ravenscar profile is uniquely defined by the tuple
-%(priority, period, WCET)%
+  induction p ; unfold Legal_protected_operation ;
+  apply Legal_PO_Body_dec.
+Qed.
 
-*)
+(*|
 
-Inductive task_kind :=
-| PERIODIC | SPORADIC | ISR.
+Semantics of Ravenscar Programs
+===============================
 
-Inductive task :=
-| Task : task_kind ->
-         identifier ->
-         priority ->
-         time -> (* period *)
-         time -> (* WCET *)
-         statements -> task.
+Reduction semantics of Ravenscar programs
+-----------------------------------------
 
-Definition A_PERIODIC_TASK :=
-  Task PERIODIC (Id "a_task") 42 10 1 Ravenscar_Cyclic_Program.
+( https://www.cs.princeton.edu/courses/archive/spr96/cs441/notes/l9.html )
 
-  (** XXX trivial checks on well-formedness possible here also ..*)
+A reduction semantics (or rewriting semantics) defines an an evaluation function eval for expressions based on a notion of reduction. We say that an expression e evaluates to an answer a if and only if e reduces to a.
 
-(**
+The reduction relation ->* is the reflexive and transitive closure of the simpler reduction relation ->. That is, ->* consists of zero or more -> steps.
+|*)
 
+Inductive red : statements * thread_state -> statements * thread_state -> Prop :=
+  | red_seq_done: forall c s,
+    red (SEQ SKIP c, s) (c, s)
 
-*)
-
-Inductive ravenscar_system :=
-| Ravenscar : list task -> list protected_object -> ravenscar_system.
-
-Definition A_RAVENSCAR_SYSTEM :=
-    Ravenscar [ A_PERIODIC_TASK ]
-              [ A_PO ].
-
-Definition po_state : Type := identifier -> nat.
-
-Inductive red : statements * nat -> statements * nat -> Prop :=
-| red_seq_comp: forall c s,
-    red (SEQ COMP c, s) (c, S s)
-| red_seq_step: forall c1 c s1 c2 s2,
+  | red_seq_step: forall c1 c s1 c2 s2,
     red (c1, s1) (c2, s2) ->
     red (SEQ c1 c, s1) (SEQ c2 c, s2)
-| red_seq_done: forall c s,
-    red (SEQ RET c, s) (c, s)
-    .
+
+  | red_comp: forall s t,
+    red (COMP t, s)
+        (SKIP, Update_CET s (COMP t))
+
+  | red_delay_until: forall s,
+      red (DELAY_UNTIL_NEXT_PERIOD, s)
+          (SKIP, Set_Next_Dispatch_Time s)
+
+  | red_po_function: forall s i1 i2,
+    red (PO_FUNCTION i1 i2, s)
+        (SKIP, Update_CET s (PO_FUNCTION i1 i2))
+
+  | red_po_entry: forall s i1 i2,
+    red (PO_ENTRY i1 i2, s)
+      (SKIP, Update_CET s (PO_ENTRY i1 i2))
+
+  | red_while_false: forall b c s,
+      beval b = false ->
+      red (WHILE b c, s) (SKIP, s)
+
+  | red_while_true: forall b c s,
+      beval b = true ->
+      red (WHILE b c, s) (SEQ c (WHILE b c), s).
+
+(*| A configuration [(c,s)] reduces to at most one configuration, in other words all Ravenscar programs are determinstic. |*)
 
 Lemma red_determ:
     forall cs cs1, red cs cs1 -> forall cs2, red cs cs2 -> cs1 = cs2.
@@ -226,9 +397,1297 @@ Proof.
     - inversion H3.
     - inversion H.
     - assert (EQ: (c2, s2) = (c4, s3)) by auto. congruence.
-    - inversion H.
-    - inversion H3.
+    - congruence.
+    - congruence.
 Qed.
 
+Lemma red_seq_steps: forall c2 s c s' c',
+  clos_refl_trans_1n _ red (c, s) (c', s') ->
+    clos_refl_trans_1n _ red ((c;;c2), s) ((c';;c2), s').
+Proof.
+  intros. dependent induction H.
+  - apply rt1n_refl.
+  - destruct y as [c1 st1]. apply rt1n_trans with (c1;;c2, st1).
+    apply red_seq_step. apply H. apply  IHclos_refl_trans_1n ; auto.
+Qed.
+
+(*|
+
+Natural semantics of Ravenscar programs
+---------------------------------------
+
+|*)
+
+Inductive rexec: thread_state -> statements -> thread_state -> Prop :=
+  | rexec_skip: forall s,
+    rexec s SKIP s
+
+  | rexec_po_function: forall s i1 i2,
+    rexec s (PO_FUNCTION i1 i2) (Update_CET s (PO_FUNCTION i1 i2))
+
+  | rexec_po_entry: forall s i1 i2,
+    rexec s (PO_ENTRY i1 i2) (Update_CET s (PO_ENTRY i1 i2))
+
+  | rexec_seq: forall c1 c2 s s' s'',
+    rexec s c1 s' -> rexec s' c2 s'' ->
+      rexec s (SEQ c1 c2) s''
+
+  | rexec_comp: forall s t,
+      rexec s (COMP t) (Update_CET s (COMP t))
+
+  | rexec_delay_until: forall s,
+      rexec s (DELAY_UNTIL_NEXT_PERIOD)
+            (Set_Next_Dispatch_Time s)
+
+  | rexec_while_false: forall b c s,
+            beval b = false ->
+            rexec s (WHILE b c) s
+
+  | rexec_while_true: forall b c s s' s'',
+            beval b = true -> rexec s c s' -> rexec s' (WHILE b c) s'' ->
+            rexec s (WHILE b c) s''.
+
+Theorem rexec_to_reds: forall s c s',
+  rexec s c s' ->
+    clos_refl_trans_1n _ red (c, s) (SKIP, s').
+Proof.
+  induction 1.
+
+  - (* SKIP *)
+    apply rt1n_refl.
+
+  - (* PO_FUNCTION *)
+    eapply rt1n_trans. apply red_po_function. apply rt1n_refl.
+
+  - (* PO_ENTRY *)
+    eapply rt1n_trans. apply red_po_entry. apply rt1n_refl.
+
+  - (* SEQ *)
+    eapply rt1n_trans'. apply red_seq_steps. apply IHrexec1.
+    eapply rt1n_trans.  apply red_seq_done.  apply IHrexec2.
+
+  - (* COMP *)
+    eapply rt1n_trans. apply red_comp. apply rt1n_refl.
+
+  - (* DELAY_UNTIL_NEXT_PERIOD *)
+    eapply rt1n_trans. apply red_delay_until. apply rt1n_refl.
+
+  - (* WHILE / false *)
+  eapply rt1n_trans. apply red_while_false. apply H. apply rt1n_refl.
+
+  - (* WHILE / true *)
+  eapply rt1n_trans. apply red_while_true. apply H.
+  eapply rt1n_trans'. apply red_seq_steps. apply IHrexec1.
+  eapply rt1n_trans. apply red_seq_done. apply IHrexec2.
+
+Qed.
+
+(*|
+Equivalence between reduction and natural semantics
+---------------------------------------------------
+|*)
+
+Lemma red_append_rexec:
+  forall c1 s1 c2 s2, red (c1, s1) (c2, s2) ->
+  forall s', rexec s2 c2 s' -> rexec s1 c1 s'.
+Proof.
+  intros until s2; intros STEP. dependent induction STEP; intros.
+
+  - (* SKIP *)
+    apply rexec_seq with s2. apply rexec_skip. auto.
+
+  - (* SEQ *)
+    inversion H; subst. apply rexec_seq with s'0.
+    eapply IHSTEP; eauto.
+    auto.
+
+  - (* COMP *)
+    inversion H. subst. apply rexec_comp.
+
+  - (* DELAY_UNTIL_NEXT_PERIOD *)
+    inversion H. subst. apply rexec_delay_until.
+
+  - (* PO_FUNCTION*)
+    inversion H. subst. apply rexec_po_function.
+
+  - (* PO_ENTRY *)
+    inversion H. subst. apply rexec_po_entry.
+
+  - (* WHILE / false *)
+    inversion H0. subst. eapply rexec_while_false. trivial.
+
+  - (* WHILE / true *)
+    inversion H0. subst. apply rexec_while_true with (s' := s'0) ; auto.
+
+Qed.
+
+(** By induction on the reduction sequence, it follows that a command
+    that reduces to [SKIP] executes according to the natural semantics,
+    with the same final state. *)
+
+Theorem reds_to_rexec: forall s c s',
+  clos_refl_trans_1n _ red (c, s) (SKIP, s') -> rexec s c s'.
+Proof.
+  intros. dependent induction H.
+  - apply rexec_skip.
+  - destruct y as [c1 s1]. apply red_append_rexec with c1 s1; auto.
+Qed.
+
+(*|
+Simulation of Ravenscar programs
+--------------------------------
+
+|*)
+
+Fixpoint Eval (fuel : nat) (st :thread_state) (s : statements)
+  : thread_state * bool
+:=
+
+  match fuel with
+  | 0 => (st, false)
+  | S fuel' =>
+
+  match s with
+    (* A sequential execution step *)
+    | COMP t => (Update_CET st s, true)
+
+    (* Operations on protected objects *)
+    | PO_FUNCTION _ _ | PO_ENTRY _ _ => (Update_CET st s, true)
+
+    (* Delay until some time *)
+    | DELAY_UNTIL_NEXT_PERIOD => (Set_Next_Dispatch_Time st, true)
+
+    | SKIP => (st, true)
+
+    | WHILE b s1 =>
+      if beval b then
+        match Eval fuel' st s1 with
+        | (st', false) => (st', false)
+        | (st', true) => Eval fuel' st' (WHILE b s1)
+        end
+      else (st, true)
+
+    | SEQ s1 s2 =>
+      match Eval fuel' st s1 with
+      | (st', false) => (st', false)
+      | (st', true) => Eval fuel' st' s2
+      end
+  end
+end.
+
+Compute Eval 10 Dummy_thread_state Ravenscar_Cyclic_Program.
+
+Lemma Eval_sound: forall fuel s c s' ,
+  Eval fuel s c = (s', true) -> rexec s c s'.
+Proof.
+  induction fuel.
+  - discriminate.
+  - induction c;  simpl.
+    + (* COMP *)
+      intros. inversion H. apply rexec_comp.
+
+    + (* PO_FUNCTION *)
+      intros. inversion H.
+      apply rexec_po_function.
+
+    + (* PO_ENTRY *)
+      intros. inversion H. apply rexec_po_entry.
+
+    + (* DELAY_UNTIL_NEXT_PERIOD *)
+      intros. inversion H. apply rexec_delay_until.
+
+    + (* SEQ *)
+      intros. destruct (Eval fuel s c1) eqn:H2.
+      apply rexec_seq with (s' := t).
+
+      apply IHfuel.
+      destruct b eqn:H0. apply H2. inversion H.
+
+      apply IHfuel.
+      destruct b eqn:H0. apply H. inversion H.
+
+    + (* WHILE *)
+      intros. destruct (beval b) eqn:H2.
+      -- destruct (Eval fuel s c) eqn:H3.
+
+        apply rexec_while_true with (s' := t).
+        apply H2.
+        apply IHfuel.
+        destruct b0. apply H3. inversion H.
+
+        apply IHfuel. destruct b0. apply H. inversion H.
+
+      -- inversion H. eapply rexec_while_false. apply H2.
+
+    + (* SKIP *) intros. inversion H. apply rexec_skip.
+Qed.
+
+(*| :coq:`Eval_cont'_end` shows that if :coq:`Eval_cont'` converges to some value, then :coq:`fuel > 0`. |*)
+Lemma Eval_end: forall fuel st s st',
+  Eval fuel st s = (st', true) -> fuel > 0.
+Proof.
+  induction fuel as [ | fuel ].
+  - discriminate.
+  - intuition.
+Qed.
+
+Lemma Eval_split_seq: forall fuel st s1 s2 st',
+  Eval (S fuel) st (s1;; s2) = (st', true) ->
+    exists st'', Eval fuel st s1 = (st'', true) /\ Eval fuel st'' s2 = (st', true).
+Proof.
+  intros.
+  simpl in H.
+  destruct (Eval fuel st s1).
+  exists t.
+  destruct b.
+  - auto.
+  - inversion H.
+Qed.
+
+Lemma Eval_split_while: forall fuel st b s1 st',
+  Eval (S fuel) st (WHILE b s1) = (st', true) ->
+    ((beval b = true) /\
+      (exists st'', (Eval fuel st s1 = (st'', true)) /\
+                    (Eval fuel st'' (WHILE b s1)) = (st', true)))
+    \/ ((beval b = false) /\ st = st').
+Proof.
+  intros.
+  simpl in H.
+  destruct (beval b).
+  - destruct (Eval fuel st s1).
+    left. split. trivial. exists t.
+    destruct b0. auto. inversion H.
+  - right. split. trivial. inversion H. trivial.
+Qed.
+
+Lemma Eval_end_fix: forall fuel st s st' ,
+  Eval fuel st s = (st', true) -> Eval (S fuel) st s = (st', true).
+Proof.
+  intro fuel.
+  induction fuel.
+  - intros. discriminate.
+  - destruct s ; try intuition. (* Simplify all trivial cases *)
+    + (* SEQ *)
+      apply Eval_split_seq in H.
+      destruct H as (st'' ,H).
+      destruct H.
+
+      assert (H1 : Eval (S (S fuel)) st (s1;; s2) =
+                match Eval (S fuel) st s1 with
+                | (st'', false) => (st'', false)
+                | (st'', true) => Eval (S fuel) st'' s2
+                end).
+      intuition.
+
+      assert (Eval (S fuel) st s1 = (st'', true)).
+      apply IHfuel ; trivial.
+      rewrite H2 in H1.
+
+      assert (Eval (S fuel) st'' s2 = (st', true)).
+      apply IHfuel ; trivial.
+
+      rewrite H3 in H1.
+      trivial.
+
+    + (* WHILE *)
+
+    assert (H1 : Eval (S (S fuel)) st (WHILE b s) =
+          if (beval b) then
+          match Eval (S fuel) st s with
+          | (st'', false) => (st'', false)
+          | (st'', true) => Eval (S fuel) st'' (WHILE b s)
+          end
+          else (st, true)).
+    intuition.
+    apply Eval_split_while in H.
+
+    destruct (beval b).
+
+    * destruct H. destruct H.
+      destruct H0 as (st'', H0).
+      destruct H0.
+
+      assert (Eval (S fuel) st s = (st'', true)).
+      apply IHfuel; trivial.
+
+      rewrite H3 in H1.
+
+      assert (Eval (S fuel) st'' (WHILE b s) = (st', true)).
+      apply IHfuel; trivial.
+
+      rewrite H4 in H1. trivial.
+
+      destruct H.
+      discriminate.
+
+    * destruct H. destruct H.
+
+      discriminate.
+
+      destruct H. subst. trivial.
+Qed.
+
+Lemma Eval_complete: forall s c s',
+  rexec s c s' -> exists fuel1,
+    forall fuel, (fuel >= fuel1)%nat -> Eval fuel s c = (s', true).
+Proof.
+  induction 1 ; intuition.
+
+  - (* SKIP *)
+    exists 1. intros.
+    assert (exists n, fuel = S n).
+    apply zero_or_succ_positive , H.
+    destruct H0 as (n, H0).
+    subst. simpl ; trivial.
+
+  - (* PO_FUNCTION *)
+    exists 1. intros.
+    assert (exists n, fuel = S n).
+    apply zero_or_succ_positive , H.
+    destruct H0 as (n, H0).
+    subst. simpl ; trivial.
+
+  - (* PO_ENTRY *)
+    exists 1. intros.
+    assert (exists n, fuel = S n).
+    apply zero_or_succ_positive , H.
+    destruct H0 as (n, H0).
+    subst. simpl ; trivial.
+
+  - (* SEQ *)
+    intros.
+    destruct IHrexec1 as (fuel1, IHrexec1').
+    destruct IHrexec2 as (fuel2, IHrexec2').
+
+    exists (fuel1 + fuel2 + 2).
+    intros.
+    assert (fuel > 0). lia.
+
+    assert (exists n, fuel = S n).
+    apply zero_or_succ_positive , H2.
+    destruct H3 as (n, H3).
+    subst. simpl.
+
+    assert (n > fuel1). lia.
+    assert (Eval n s c1 = (s', true)). apply IHrexec1'. lia.
+    rewrite H4.
+    apply IHrexec2'. lia.
+
+  - (* COMP *)
+    exists 1. intros.
+    assert (exists n, fuel = S n).
+    apply zero_or_succ_positive , H.
+    destruct H0 as (n, H0).
+    subst. simpl ; trivial.
+
+  - (* DELAY_UNTIL_NEXT_PERIOD *)
+    exists 1. intros.
+    assert (exists n, fuel = S n).
+    apply zero_or_succ_positive , H.
+    destruct H0 as (n, H0).
+    subst. simpl ; trivial.
+
+  - (* WHILE / false *)
+    exists 1. intros.
+    assert (exists n, fuel = S n).
+    apply zero_or_succ_positive , H0.
+    destruct H1 as (n, H1).
+    subst. simpl. rewrite H. trivial.
+
+  - (* WHILE / true *)
+
+    destruct IHrexec1 as (fuel1, IHrexec1').
+    destruct IHrexec2 as (fuel2, IHrexec2').
+
+    exists (fuel1 + fuel2 + 2).
+    intros.
+    assert (fuel > 0). lia.
+
+    assert (exists n, fuel = S n).
+    apply zero_or_succ_positive , H3.
+    destruct H4 as (n, H4).
+    subst. simpl.
+    rewrite H.
+
+    assert (n > fuel1). lia.
+    assert (Eval n s c = (s', true)). apply IHrexec1'. lia.
+    rewrite H5. apply IHrexec2'. lia.
+Qed.
+
+(*|
+Continuation semantics
+======================
+
+we now introduce another form of "small-step" semantics as an alternative to the reduction semantics.  In the new semantics, the command to be executed is explicitly decomposed into
+
+  * a sub-command under focus, where computation takes place;
+  * a context that describes the position of the sub-command in the
+      whole command; or, equivalently, a continuation that describes
+      the parts of the whole command that remain to execute once
+      the sub-command terminates.
+
+Consequently, the semantics is presented as a transition relation between triples (sub-command under focus, continuation, state).
+
+|*)
+
+Inductive cont : Type :=
+  | Kstop
+  | Kseq (c: statements) (k: cont)
+  | Kwhile (b: bexp) (c: statements) (k: cont).
+
+Fixpoint statement_to_cont (c : statements) :=
+  match c with
+  | SEQ c1 c2 => Kseq c1 (statement_to_cont c2)
+  | WHILE b c1 => Kwhile b c1 Kstop
+  | c => Kseq c Kstop
+  end.
+
+Fixpoint cont_to_statement (k: cont) (c: statements) :=
+  match k with
+    | Kstop => c
+    | Kseq c1 k1 => cont_to_statement k1 (SEQ c c1)
+    | Kwhile b1 c1 k1 => cont_to_statement k1 (SEQ c (WHILE b1 c1))
+  end.
+
+Inductive step: statements * cont * thread_state ->
+                statements * cont * thread_state -> Prop :=
+
+  | step_seq: forall c1 c2 s k,               (**r focusing *)
+      step (SEQ c1 c2, k, s) (c1, Kseq c2 k, s)
+
+  | step_skip_seq: forall c k s,              (**r resumption *)
+      step (SKIP, Kseq c k, s) (c, k, s)
+
+  | step_comp: forall t k s,
+      step (COMP t, k, s)
+            (SKIP, k,
+              (Update_CET s (COMP t)))
+
+  | step_delay_until: forall k s ,
+    step (DELAY_UNTIL_NEXT_PERIOD, k, s)
+          (SKIP, k,
+            (Set_Next_Dispatch_Time s))
+
+  | step_po_function: forall c1 c2 k s ,
+    step (PO_FUNCTION c1 c2, k, s)
+        (SKIP, k, (Update_CET s (PO_FUNCTION c1 c2)))
+
+  | step_po_entry: forall c1 c2 k s ,
+    step (PO_ENTRY c1 c2, k, s)
+          (SKIP, k, (Update_CET s (PO_ENTRY c1 c2)))
+
+  | step_while_done: forall b c k s,          (**r computation *)
+    beval b = false ->
+      step (WHILE b c, k, s) (SKIP, k, s)
+
+  | step_while_loop: forall b c k s,          (**r computation + focusing *)
+    beval b = true ->
+      step (WHILE b c, k, s) (c, Kwhile b c k, s).
+
+(*|
+Equivalence between the continuation semantics and the reduction semantics
+--------------------------------------------------------------------------
+|*)
+
+Inductive match_conf : statements * cont * thread_state -> statements * thread_state -> Prop :=
+  | match_conf_intro: forall c k s c',
+      c' = cont_to_statement k c ->
+      match_conf (c, k, s) (c', s).
+
+(*| We show that every transition of the continuation semantics
+    is simulated by zero, one or several reduction steps.
+    The anti-stuttering measure counts the nesting of [SEQ] constructs
+    in the command. |*)
+
+Fixpoint num_seq (c: statements) : nat :=
+  match c with
+  | SEQ c1 c2 => S (num_seq c1)
+  | _ => O
+  end.
+
+Definition kmeasure (C: statements * cont * thread_state ) : nat :=
+  let '(c, k, s) := C in num_seq c.
+
+Remark red_cont_to_statement:
+  forall k c1 s1 c2 s2,
+  red (c1, s1) (c2, s2) ->
+  red (cont_to_statement k c1, s1) (cont_to_statement k c2, s2).
+Proof.
+  induction k; intros; simpl; eauto using red_seq_step.
+Qed.
+
+Lemma simulation_cont_red:
+  forall C1 C1', step C1 C1' ->
+  forall C2, match_conf C1 C2 ->
+  exists C2',
+     (clos_refl_trans_1n_plus _ red C2 C2' \/
+     (clos_refl_trans_1n _ red C2 C2' /\ kmeasure C1' < kmeasure C1))%nat
+  /\ match_conf C1' C2'.
+  Proof.
+    destruct 1; intros C2 MC; inversion MC; subst; cbn.
+    1: econstructor; split; [right; split; [apply rt1n_refl | lia] | constructor; auto ].
+
+    all: econstructor; split; [left; apply clos_refl_trans_1n_plus_one; apply red_cont_to_statement; auto using red | constructor; auto].
+Qed.
+
+Inductive red_cont_to_statement_cases:
+  cont -> statements -> thread_state -> statements -> thread_state -> Prop :=
+  | racc_base: forall c1 s1 c2 s2 k,
+    red (c1, s1) (c2, s2) ->
+    red_cont_to_statement_cases k c1 s1 (cont_to_statement k c2) s2
+  | racc_skip_seq: forall c k s,
+    red_cont_to_statement_cases (Kseq c k) SKIP s (cont_to_statement k c) s
+  | racc_skip_while: forall b c k s,
+  red_cont_to_statement_cases (Kwhile b c k) SKIP s (cont_to_statement k (WHILE b c)) s.
+
+Lemma invert_red_cont_to_statement:
+  forall k c s c' s',
+    red (cont_to_statement k c, s) (c', s') ->
+    red_cont_to_statement_cases k c s c' s'.
+Proof.
+  induction k; simpl; intros.
+  - (* Kstop *)
+    change c' with (cont_to_statement Kstop c'). apply racc_base; auto.
+  - (* Kseq *)
+    specialize (IHk _ _ _ _ H). inversion IHk; subst.
+    + (* base *)
+    inversion H0; clear H0; subst.
+      * (* seq finish *)
+        apply racc_skip_seq.
+      * (* seq step *)
+        change (cont_to_statement k (c4;;c)) with (cont_to_statement (Kseq c k) c4).
+        apply racc_base; auto.
+
+  - (* KWhile *)
+  specialize (IHk _ _ _ _ H). inversion IHk; subst.
+  inversion H0; clear H0; subst.
+    * (* seq finish *)
+      apply racc_skip_while.
+    * (* seq step *)
+      change (cont_to_statement k (c4;;WHILE b c)) with (cont_to_statement(Kwhile b c k) c4).
+      apply racc_base; auto.
+Qed.
+
+(*|
+Simulation in the continuation style
+------------------------------------
+|*)
+
+Definition Initial_thread_state (p : Time):=
+  {| th_state := READY ;
+     th_period := p ;
+     th_cet := 0 ;
+     th_next_dispatch := 0 |}.
+
+Example Test_Program_1 := COMP 1 ;; SKIP ;; COMP 2 ;; SKIP ;; COMP 3.
+Check Test_Program_1.
+
+Fixpoint Eval_cont' (fuel : nat) (st :thread_state) (k : cont)
+  : thread_state * cont
+:=
+  match fuel with
+  | 0 => (st, k)
+  | S n =>
+    match k with
+    | Kstop => (st, Kstop)
+
+    | Kseq s' k' =>
+      match Eval n st s' with
+      | (st', false) => (st, k)
+      | (st', true) => Eval_cont' n st' k'
+      end
+
+    | Kwhile b s' k' =>
+      if beval b then
+          match Eval n st s' with
+          | (st', false) => (st, (Kseq s' (Kwhile b s' k')))
+          | (st', true) => Eval_cont' n st' (Kwhile b s' k')
+          end
+      else (st, Kstop)
+    end
+end.
+
+Compute Eval_cont' 10 Dummy_thread_state
+  (statement_to_cont Ravenscar_Cyclic_Program).
+
+(*| :coq:`Eval_cont'_end` shows that if :coq:`Eval_cont'` converges to some value, then :coq:`fuel > 0`. |*)
+
+Lemma Eval_cont'_end: forall k st x fuel, k <> Kstop ->
+  Eval_cont' fuel st k = (x, Kstop) -> fuel > 0.
+Proof.
+  induction fuel as [ | fuel ].
+  - simpl. intros H H0. inversion H0. contradiction.
+  - intuition.
+Qed.
+
+Lemma Eval_cont'_end': forall fuel k st x ,
+  Eval_cont' fuel st k = (x, Kstop) ->
+    Eval_cont' (S fuel) st k = (x, Kstop).
+Proof.
+  intro fuel.
+  induction fuel.
+  - intros. simpl in *. inversion H. trivial.
+  - destruct k.
+    + (* Kstop *)
+      intuition.
+
+    + (* Kseq *)
+      intros. simpl in H.
+
+      assert (H0: exists st', Eval fuel st c = (st', true)).
+      destruct (Eval fuel st c).
+      exists t ; trivial.
+      destruct b. trivial. inversion H.
+
+      destruct H0 as (st', H0).
+      rewrite H0 in H.
+
+      assert (H1: Eval_cont' (S (S fuel)) st (Kseq c k) =
+        match Eval (S fuel) st c with
+          | (st', false) => (st, (Kseq c k))
+          | (st', true) => Eval_cont' (S fuel) st' k
+        end).
+      reflexivity.
+
+      assert (H2: Eval (S fuel) st c = (st', true)).
+      apply Eval_end_fix. apply H0.
+
+      rewrite H2 in H1.
+
+      assert (H3: Eval_cont' (S fuel) st' k = (x, Kstop)).
+      apply IHfuel. apply H.
+
+      rewrite H3 in H1. trivial.
+
+    + (* Kwhile *)
+      intros. simpl in H.
+
+      assert (H0: Eval_cont' (S (S fuel)) st (Kwhile b c k) =
+        if beval b
+        then
+        match Eval (S fuel) st c with
+        | (st', false) => (st, (Kseq c (Kwhile b c k)))
+        | (st', true) => Eval_cont' (S fuel) st' (Kwhile b c k)
+  end
+        else (st, Kstop)
+      ). reflexivity.
+
+      destruct (beval b) eqn:Hbeval.
+
+      * assert (H1: exists st', Eval fuel st c = (st', true)).
+        destruct (Eval fuel st c).
+        exists t ; trivial.
+        inversion H.
+        destruct b0. trivial. inversion H2.
 
 
+        destruct H1 as (st', H1).
+        rewrite H1 in H.
+
+        assert (H2: Eval (S fuel) st c = (st', true)).
+        apply Eval_end_fix. apply H1.
+        rewrite H2 in H0.
+
+        assert (Eval_cont' (S fuel) st' (Kwhile b c k) = (x, Kstop)).
+        apply IHfuel. apply H.
+        rewrite H3 in H0. trivial.
+
+      * rewrite H in H0. trivial.
+Qed.
+
+Lemma Eval_cont'_Kstop: forall fuel st ,
+  fuel > 0 -> Eval_cont' fuel st Kstop = (st, Kstop).
+Proof.
+  intros.
+  assert (exists n, fuel = S n).
+  apply zero_or_succ_positive, H.
+  destruct H0 as (n, H0).
+  subst.
+  simpl.
+  reflexivity.
+Qed.
+
+Lemma statement_to_cont_no_Kstop:
+  forall s, (exists s' k', statement_to_cont s = Kseq s' k') \/
+    (exists b s' k', statement_to_cont s = Kwhile b s' k').
+Proof.
+  intros.
+  induction s ; simpl.
+  1-5,7: left ; eexists ; eexists ; trivial.
+  right. exists b; exists s; exists Kstop ; trivial.
+Qed.
+
+Lemma statement_to_cont_no_Kstop':
+  forall s, statement_to_cont s <> Kstop.
+Proof.
+  intros.
+  induction s ; discriminate.
+Qed.
+
+Lemma Eval_cont'_Eval_OK: forall fuel s st x,
+  Eval_cont' fuel st (statement_to_cont s) = (x, Kstop)
+  -> Eval fuel st s = (x, true).
+Proof.
+  (* This proof is technical but not that complex.
+      We perform a double induction on fuel and s (statements). *)
+
+  intro fuel.
+  induction fuel.
+
+- (* fuel = 0 *)
+  intros. simpl.
+
+  (* We have an apparent contradiction in H, that we leverage to
+    complete the proof. *)
+  inversion H. subst.
+  assert (statement_to_cont s <> Kstop).
+  apply statement_to_cont_no_Kstop'. contradiction.
+
+- (* S fuel *)
+  intro s.
+  induction s.
+
+  + (* s = COMP *)
+    intros.
+
+    (* Intermediate result #1 *)
+    assert (H1: exists st', Eval fuel st (COMP WCET) = (st', true)).
+    destruct (Eval fuel st (COMP WCET)) eqn:H2.
+    simpl in H. rewrite H2 in H. exists t.
+    destruct b. trivial. inversion H.
+
+    destruct H1 as (st', H1).
+
+    (* Intermediate result #2 *)
+    assert (H2: Eval_cont' fuel st' Kstop  = (st', Kstop)).
+    destruct fuel; simpl ; trivial.
+
+    (* We now show that st' = x *)
+    assert (H3: st' = x).
+    simpl in H. rewrite H1 in H.
+    rewrite H2 in H. inversion H. trivial.
+
+    subst.
+    apply Eval_end_fix. trivial.
+
+  + (* s = PO_FUNCTION po op *)
+    intros.
+
+    (* Intermediate result #1 *)
+    assert (H1: exists st',
+      Eval fuel st (PO_FUNCTION po op) = (st', true)).
+    destruct (Eval fuel st (PO_FUNCTION po op)) eqn:H2.
+    simpl in H. rewrite H2 in H. exists t.
+    destruct b. trivial. inversion H.
+
+    destruct H1 as (st', H1).
+
+    (* Intermediate result #2 *)
+    assert (H2: Eval_cont' fuel st' Kstop  = (st', Kstop)).
+    destruct fuel; simpl ; trivial.
+
+    (* We now show that st' = x *)
+    assert (H3: st' = x).
+    simpl in H. rewrite H1 in H.
+    rewrite H2 in H. inversion H. trivial.
+
+    subst.
+    apply Eval_end_fix. trivial.
+
+  + (* s = PO_ENTRY po op *)
+    intros.
+
+    (* Intermediate result #1 *)
+    assert (H1: exists st',
+      Eval fuel st (PO_ENTRY po op) = (st', true)).
+    destruct (Eval fuel st (PO_ENTRY po op)) eqn:H2.
+    simpl in H. rewrite H2 in H. exists t.
+    destruct b. trivial. inversion H.
+
+    destruct H1 as (st', H1).
+
+    (* Intermediate result #2 *)
+    assert (H2: Eval_cont' fuel st' Kstop  = (st', Kstop)).
+    destruct fuel; simpl ; trivial.
+
+    (* We now show that st' = x *)
+    assert (H3: st' = x).
+    simpl in H. rewrite H1 in H.
+    rewrite H2 in H. inversion H. trivial.
+
+    subst.
+    apply Eval_end_fix. trivial.
+
+  + (* s = DELAY_UNTIL_NEXT_PERIOD *)
+    intros.
+
+    (* Intermediate result #1 *)
+    assert (H1: exists st',
+      Eval fuel st DELAY_UNTIL_NEXT_PERIOD = (st', true)).
+    destruct (Eval fuel st DELAY_UNTIL_NEXT_PERIOD) eqn:H2.
+    simpl in H. rewrite H2 in H. exists t.
+    destruct b. trivial. inversion H.
+
+    destruct H1 as (st', H1).
+
+    (* Intermediate result #2 *)
+    assert (H2: Eval_cont' fuel st' Kstop  = (st', Kstop)).
+    destruct fuel; simpl ; trivial.
+
+    (* We now show that st' = x *)
+    assert (H3: st' = x).
+    simpl in H. rewrite H1 in H.
+    rewrite H2 in H. inversion H. trivial.
+
+    subst.
+    apply Eval_end_fix. trivial.
+
+  + (* s = s1 ;; s2 *)
+    intros. simpl in H. simpl.
+
+    assert (H1: exists st',  Eval fuel st s1 = (st', true)).
+    destruct (Eval fuel st s1) eqn:H2.
+    exists t. destruct b. trivial. inversion H.
+
+    destruct H1 as (st', H1).
+    rewrite H1 in H.
+    rewrite H1.
+
+    eapply IHfuel. apply H.
+
+  + (* s = WHILE b s *)
+
+    intros.
+
+    simpl in H. simpl.
+    destruct (beval b) eqn:beval.
+    * (* beval b = true *)
+
+      assert (H1: exists st',  Eval fuel st s = (st', true)).
+      destruct (Eval fuel st s) eqn:H2.
+      exists t. destruct b0. trivial. inversion H.
+
+      destruct H1 as (st', H1).
+      rewrite H1 in H.
+      rewrite H1.
+
+      apply IHfuel.
+
+      assert (H2: statement_to_cont (WHILE b s) = Kwhile b s Kstop).
+      trivial.
+      rewrite H2.
+      apply H.
+
+    * (* beval b = false *)
+      inversion H. trivial.
+
+  +(* s = SKIP *)
+    intros.
+
+    (* Intermediate result #1 *)
+    assert (H1: exists st', Eval fuel st (SKIP) = (st', true)).
+    destruct (Eval fuel st (SKIP)) eqn:H2.
+    simpl in H. rewrite H2 in H. exists t.
+    destruct b. trivial. inversion H.
+
+    destruct H1 as (st', H1).
+
+    (* Intermediate result #2 *)
+    assert (H2: Eval_cont' fuel st' Kstop  = (st', Kstop)).
+    destruct fuel; simpl ; trivial.
+
+    (* We now show that st' = x *)
+    assert (H3: st' = x).
+    simpl in H. rewrite H1 in H.
+    rewrite H2 in H. inversion H. trivial.
+
+    subst.
+    apply Eval_end_fix. trivial.
+
+Qed.
+
+Lemma Eval_Eval_cont'_OK: forall fuel s st x,
+  (Eval fuel st s = (x, true) ->
+    Eval_cont' fuel st (statement_to_cont s) = (x, Kstop))
+\/
+  (Eval fuel st s = (x, false) ->
+    Eval_cont' fuel st (statement_to_cont s) <> (x, Kstop)).
+Proof.
+  intro fuel.
+  induction fuel.
+  - (* fuel = 0 *)
+    intros. simpl. right. intros. inversion H.
+
+    assert (H0: statement_to_cont s <> Kstop).
+    apply statement_to_cont_no_Kstop'.
+
+    rewrite pair_equal_spec. firstorder.
+
+  - (* S fuel *)
+    intro s. induction s.
+
+    + (* s = COMP WCET *)
+      pose (s':= COMP WCET).
+
+      intros. simpl.
+      destruct (Eval fuel st s') eqn:Hs.
+      destruct b.
+
+      * (* b = true *)
+        left.
+
+        assert (Hfuel: fuel > 0).
+        apply Eval_end with (st := st) (s := s') (st' := t).
+        apply Hs.
+
+        assert (Hn: exists n, fuel = S n).
+        apply zero_or_succ_positive, Hfuel.
+        destruct Hn as (n, Hn).
+
+        subst.
+        simpl.
+        repeat rewrite pair_equal_spec. firstorder.
+
+      * (* b = false *)
+        right. intros. inversion H.
+
+
+    + (* s = PO_FUNCTION po op*)
+      pose (s':= PO_FUNCTION po op).
+
+      intros. simpl.
+      destruct (Eval fuel st s') eqn:Hs.
+      destruct b.
+
+      * (* b = true *)
+        left.
+
+        assert (Hfuel: fuel > 0).
+        apply Eval_end with (st := st) (s := s') (st' := t).
+        apply Hs.
+
+        assert (Hn: exists n, fuel = S n).
+        apply zero_or_succ_positive, Hfuel.
+        destruct Hn as (n, Hn).
+
+        subst.
+        simpl.
+        repeat rewrite pair_equal_spec. firstorder.
+
+      * (* b = false *)
+        right. intros. inversion H.
+
+    + (* s = PO_ENTRY po op*)
+      pose (s':= PO_ENTRY po op).
+
+      intros. simpl.
+      destruct (Eval fuel st s') eqn:Hs.
+      destruct b.
+
+      * (* b = true *)
+        left.
+
+        assert (Hfuel: fuel > 0).
+        apply Eval_end with (st := st) (s := s') (st' := t).
+        apply Hs.
+
+        assert (Hn: exists n, fuel = S n).
+        apply zero_or_succ_positive, Hfuel.
+        destruct Hn as (n, Hn).
+
+        subst.
+        simpl.
+        repeat rewrite pair_equal_spec. firstorder.
+
+      * (* b = false *)
+        right. intros. inversion H.
+
+    + (* s = DELAY_UNTIL_NEXT_PERIOD*)
+      pose (s':= DELAY_UNTIL_NEXT_PERIOD).
+
+      intros. simpl.
+      destruct (Eval fuel st s') eqn:Hs.
+      destruct b.
+
+      * (* b = true *)
+        left.
+
+        assert (Hfuel: fuel > 0).
+        apply Eval_end with (st := st) (s := s') (st' := t).
+        apply Hs.
+
+        assert (Hn: exists n, fuel = S n).
+        apply zero_or_succ_positive, Hfuel.
+        destruct Hn as (n, Hn).
+
+        subst.
+        simpl.
+        repeat rewrite pair_equal_spec. firstorder.
+
+      * (* b = false *)
+        right. intros. inversion H.
+
+    + (* s = s1 ;; s2 *)
+      intros. simpl.
+      destruct (Eval fuel st s1) eqn:Hs1.
+      destruct b.
+
+      * apply IHfuel.
+      * right. intros. rewrite pair_equal_spec. intuition. inversion H2.
+
+    + (* s = WHILE b s *)
+      intros. simpl.
+      destruct (beval b) eqn:beval.
+      destruct (Eval fuel st s) eqn:Hs.
+      destruct b0.
+      * apply IHfuel.
+      * right. intros. rewrite pair_equal_spec. intuition. inversion H2.
+      * left. intros. inversion H. trivial.
+
+    + (* S = SKIP *)
+
+    pose (s':= SKIP).
+
+    intros. simpl.
+    destruct (Eval fuel st s') eqn:Hs.
+    destruct b.
+
+    * (* b = true *)
+      left.
+
+      assert (Hfuel: fuel > 0).
+      apply Eval_end with (st := st) (s := s') (st' := t).
+      apply Hs.
+
+      assert (Hn: exists n, fuel = S n).
+      apply zero_or_succ_positive, Hfuel.
+      destruct Hn as (n, Hn).
+
+      subst.
+      simpl.
+      repeat rewrite pair_equal_spec. firstorder.
+
+    * (* b = false *)
+      right. intros. inversion H.
+Qed.
+
+Fixpoint Trace_Eval_Cont''
+  (n : nat)
+  (st_k : (thread_state * cont))
+  (l : list (thread_state * cont))
+  : list (thread_state * cont)
+:=
+  match n with
+  | 0 => l
+  | S n' =>
+  let (st, k) := st_k in
+    let x := Eval_cont' 1 st k in
+      match x with
+        | (st', Kstop) => l ++ [(st', Kstop)]
+        | (st', k') =>
+          Trace_Eval_Cont'' n' (st', k') (l ++ [(st', k')])
+      end
+  end.
+
+Fact Run_Test_Program_0_OK' :
+  Eval_cont' 10 (Initial_thread_state 0) (statement_to_cont Test_Program_1) =
+  ({| th_state := READY; th_period := 0 ; th_cet := 6 ; th_next_dispatch := 0 |}, Kstop).
+Proof. trivial. Qed.
+
+Compute Eval_cont' 3 (Initial_thread_state 0) (statement_to_cont Test_Program_1).
+
+Compute Trace_Eval_Cont'' 10
+  ((Initial_thread_state 0), (statement_to_cont Test_Program_1)) [].
+
+
+(*|
+Simulation of Ravenscar tasksets
+================================
+
+|*)
+
+Inductive task_instance :=
+| task_i: identifier -> priority -> thread_state -> cont -> task_instance.
+Scheme Equality for task_instance.
+
+Definition Map_Task_to_Task_Instance (t : task) :=
+  match t with
+  | Task kind ident priority period statements =>
+    task_i ident priority (Initial_thread_state period) (statement_to_cont statements)
+  end.
+
+Definition Idle_task_Instance := Map_Task_to_Task_Instance IDLE_TASK.
+Compute Idle_task_Instance.
+
+Definition get_id (i : task_instance) :=
+  match i with
+  | task_i id _ _ _ => id
+  end.
+
+Definition get_priority (i : task_instance) : nat :=
+  match i with
+  | task_i _ priority _ _ => priority
+  end.
+Definition get_task_state (i : task_instance) :=
+  match i with
+  | task_i _ _ st _ => st.(th_state)
+  end.
+
+Definition get_thread_state_and_cont (i : task_instance) :=
+  match i with
+  | task_i _ _ st k => (st, k)
+  end.
+
+Definition get_thread_state (i : task_instance) :=
+  match i with
+  | task_i _ _ st _ => st
+  end.
+
+Definition get_continuation (i : task_instance) :=
+  match i with
+  | task_i _ _ _ k => k
+  end.
+
+Definition reset_cet (i : task_instance) :=
+  match i with
+  | task_i id p st k => task_i id p (reset_thread_cet st) k
+  end.
+
+Definition Simulate_Task (i : task_instance) (fuel : nat) : task_instance :=
+  let (st, k) := Eval_cont' fuel (get_thread_state i) (get_continuation i) in
+  match (st, k) with
+  | (st, Kstop) =>
+      task_i (get_id i) (get_priority i) (set_thread_state st IDLE) k
+  | (st, k) => task_i (get_id i) (get_priority i) st k
+
+  end.
+
+Definition max_prio_thread (i1 i2: task_instance) :=
+  if (negb (task_state_beq (get_task_state i1) READY)) &&
+     (negb (task_state_beq (get_task_state i2) READY))
+  then Idle_task_Instance
+
+  else if (task_state_beq (get_task_state i1) READY) &&
+          (negb (task_state_beq (get_task_state i2) READY))
+  then i1
+
+  else if (negb (task_state_beq (get_task_state i1) READY)) &&
+          (task_state_beq (get_task_state i2) READY)
+  then i2
+
+  else if Nat.leb (get_priority i2) (get_priority i1)
+  then i1
+
+  else i2.
+
+Definition get_thread_by_priority (l : list task_instance) :=
+  match l with
+  | [] => Idle_task_Instance
+  | h :: t => fold_left (fun acc x => max_prio_thread acc x) l h
+  end.
+
+Definition get_next_dispatch_time_i (i : task_instance) :=
+  th_next_dispatch (get_thread_state i).
+
+Definition get_next_dispatch_time_l (l : list task_instance) :=
+  list_min (map (fun x => get_next_dispatch_time_i x) l).
+
+Definition update_thread_state_at_time (i : task_instance) (t : Time) :=
+  match i with
+  | task_i id p st k =>
+    if (PeanoNat.Nat.eqb (th_next_dispatch st) t) then
+      task_i id p (set_thread_state st READY) k
+    else
+      i
+  end.
+
+Definition update_all_thread_state_at_time
+  (l : list task_instance)
+  (t : Time)
+:=
+  map (fun x => update_thread_state_at_time x t) l.
+
+Fixpoint replace_task_instance (i : task_instance) (l : list task_instance) :=
+  match l with
+  | [] => []
+  | h :: t => if (identifier_beq (get_id i) (get_id h))
+              then i :: t
+              else h :: (replace_task_instance i t)
+  end.
+
+(*|
+System
+-------
+|*)
+
+Record ravenscar_system := {
+  clock : Time ;
+  taskset : list task_instance ;
+}.
+
+(*|
+
+:coq:`Simulate_Ravenscar_Monocore` simulate a Ravenscar system, for the mono core case. It proceeds in a basic sequence of actions to
+
+* elect the next thread to be executed
+* run this thread
+* from the state of the thread, increase the global clock by the thread cet
+* reset the cet of the thread
+* update the task set.
+
+|*)
+
+Definition Simulate_Ravenscar_Monocore (s : ravenscar_system) (fuel : nat) :=
+  let l := taskset s in
+  let elected_thread := get_thread_by_priority l in
+
+  if (negb (task_instance_beq Idle_task_Instance elected_thread)) then
+    let executed_thread := Simulate_Task elected_thread fuel in
+    let time_advance := th_cet (get_thread_state executed_thread) in
+    let executed_thread' := reset_cet executed_thread in {|
+      clock := (clock s) + time_advance;
+      taskset := replace_task_instance executed_thread' l;
+    |}
+  else
+    let next_dispatch := get_next_dispatch_time_l l in {|
+      clock := next_dispatch ;
+      taskset := update_all_thread_state_at_time l next_dispatch;
+    |}.
+
+(*|
+Examples
+========
+
+|*)
+
+Unset Printing Records. (* condensed printing for records *)
+
+Example A_PERIODIC_TASK_1 :=
+  Task PERIODIC (Id "task_1") 1 10 Ravenscar_Cyclic_Program.
+
+Example A_PERIODIC_TASK_2 :=
+  Task PERIODIC (Id "task_2") 2 10 Ravenscar_Cyclic_Program.
+
+Example TASK_1 := Map_Task_to_Task_Instance A_PERIODIC_TASK_1.
+Example TASK_2 := Map_Task_to_Task_Instance A_PERIODIC_TASK_2.
+
+Print Simulate_Task.
+
+Compute Simulate_Task TASK_1 10.
+
+Example system_1 := {|
+  clock := 0;
+  taskset := [TASK_1 ; TASK_2 ];
+|}.
+
+Example system_1_10 := Simulate_Ravenscar_Monocore system_1 10.
+Compute system_1_10.
+
+Example system_1_20 := Simulate_Ravenscar_Monocore system_1_10 20.
+Compute system_1_20.
+
+Example system_1_30 := Simulate_Ravenscar_Monocore system_1_20 30.
+Compute system_1_30.
+
+Example system_1_40 := Simulate_Ravenscar_Monocore system_1_30 30.
+Compute system_1_40.
